src/ConcreteEvidence.v
@@ -17,8 +17,7 @@ Inductive EvidenceC: Set :=
 (*
 | nnc: N_ID -> BS -> EvidenceC -> EvidenceC *)
 | ssc: EvidenceC -> EvidenceC -> EvidenceC
-(*| ppc: EvidenceC -> EvidenceC -> EvidenceC 
-*).
+| ppc: EvidenceC -> EvidenceC -> EvidenceC.
 
 
 (*
@@ -56,12 +55,10 @@ Inductive Ev_Shape: EvidenceC -> Evidence -> Prop :=
     Ev_Shape e1 e1t ->
     Ev_Shape e2 e2t ->
     Ev_Shape (ssc e1 e2) (ss e1t e2t)
-             (*
 | ppt: forall e1 e2 e1t e2t,
     Ev_Shape e1 e1t ->
     Ev_Shape e2 e2t ->
-    Ev_Shape (ppc e1 e2) (pp e1t e2t)
-*).
+    Ev_Shape (ppc e1 e2) (pp e1t e2t).
 Hint Constructors Ev_Shape : core.
 
 Ltac evShapeFacts :=
@@ -79,9 +76,8 @@ Ltac evShapeFacts :=
   | [H: Ev_Shape _ (nn _ _) |- _] => invc H *)
   | [H: Ev_Shape (ssc _ _) _ |- _] => invc H
   | [H: Ev_Shape _ (ss _ _) |- _] => invc H
-  (*| [H: Ev_Shape (ppc _ _) _ |- _] => invc H
+  | [H: Ev_Shape (ppc _ _) _ |- _] => invc H
   | [H: Ev_Shape _ (pp _ _) |- _] => invc H 
-   *)
   end.
 
 
