src/Impl_vm.v
@@ -32,7 +32,7 @@ Fixpoint build_comp (t:AnnoTerm): VM unit :=
     e2r <- get_ev ;;
     put_ev (ssc e1r e2r) ;;
     add_tracem [Term.join (Nat.pred y) p]
-(*
+
   | abpar (x,y) (sp1,sp2) t1 t2 =>
     e <- get_ev ;;
     p <- get_pl ;;
@@ -58,7 +58,6 @@ Fixpoint build_comp (t:AnnoTerm): VM unit :=
     e2r <- get_store_at loc2 ;;
     put_ev (ppc e1r e2r) ;;
     add_tracem [Term.join (Nat.pred y) p]
- *)
   end.
 
 Definition run_vm (t:AnnoTerm) st : vm_st :=
